pulse/share/steel/examples/pulse/dice/dpe/DPE.fst
@@ -37,8 +37,8 @@ open Pulse.Lib.BoundedIntegers
 open Pulse.Lib.OnRange
 open Pulse.Lib.HashTable.Type
 
-assume
-val run_stt (#a:Type) (#post:a -> vprop) (f:stt a emp post) : a
+// assume
+// val run_stt (#a:Type) (#post:a -> vprop) (f:stt a emp post) : a
 
 (* Global State *)
 
@@ -53,10 +53,18 @@ type session_state =
   | SessionError //error description
 
 
+//
+// These two definitions extract to non-exhaustive patterns in Rust
+//   which fails to typecheck
+//
+
+noextract
 let ctxt_of (s:session_state { Available? s })
   : context_t
-  = let Available { context } = s in context
+  = let Available {context} = s in
+    context
 
+noextract
 let hndl_of (s:session_state { Available? s })
   : ctxt_hndl_t
   = let Available { handle } = s in handle
@@ -75,6 +83,7 @@ let session_state_perm (s:session_state) =
     exists* repr. context_perm (ctxt_of s) repr
 
 let mk_available_payload handle context = { handle; context }
+
 ```pulse
 fn intro_session_state_perm_available 
       (ctxt:context_t)
@@ -108,6 +117,9 @@ fn elim_session_state_perm_available (s:(s:session_state { Available? s }))
 }
 ```
 
+// Marking this noextract since this spec only
+// What will krml do?
+noextract
 let session_table_map = PHT.pht_t sid_t session_state
 
 let session_perm (stm:session_table_map) (sid:nat) =
@@ -117,60 +129,84 @@ let session_perm (stm:session_table_map) (sid:nat) =
        | None -> emp
        | Some s -> session_state_perm s
 
-let global_state_lock_pred
-  (session_id_counter: R.ref sid_t)
-  (session_table: R.ref (ht_t sid_t session_state))
-: vprop
-= exists* ht stm sid.
-    pts_to session_id_counter sid **
-    pts_to session_table ht **
-    models ht stm **
-    on_range (session_perm stm) 0 (U32.v sid)
-  
 noeq
 type global_state_t = {
-  session_id_counter: R.ref sid_t;
-  session_table: R.ref (ht_t sid_t session_state);
-  lock: L.lock (global_state_lock_pred session_id_counter session_table)
+  session_id_counter:sid_t;
+  session_table:ht_t sid_t session_state;
+  // lock: L.lock (global_state_lock_pred session_id_counter session_table)
 }
-let mk_global_state
-      (sid_counter:R.ref sid_t)
-      (session_table:R.ref (ht_t sid_t session_state))
-      (lock:L.lock (global_state_lock_pred sid_counter session_table))
-: global_state_t
-= { session_id_counter = sid_counter;
-    session_table = session_table;
-    lock = lock }
 
-assume Fits_size_t_u32 : squash (US.fits_u32)
-let sid_hash (x:sid_t) : US.t = US.of_u32 x
+let global_state_mutex_pred (gst:option global_state_t) : vprop =
+  match gst with
+  | None -> emp
+  | Some gst ->
+    exists* stm.
+      models gst.session_table stm **
+      on_range (session_perm stm) 0 (U32.v gst.session_id_counter)
 
-#push-options "--ext 'pulse:env_on_err' --print_implicits"
+// let mk_global_state
+//       (sid_counter:R.ref sid_t)
+//       (session_table:R.ref (ht_t sid_t session_state))
+//       (lock:L.lock (global_state_lock_pred sid_counter session_table))
+// : global_state_t
+// = { session_id_counter = sid_counter;
+//     session_table = session_table;
+//     lock = lock }
+
+// TODO: Uncomment it
+// assume Fits_size_t_u32 : squash (US.fits_u32)
+// TODO: add support for extracting closures
+// #push-options "--admit_smt_queries true --warn_error -342"
+// let sid_hash (x:sid_t) : US.t = US.of_u32 x
+// #pop-options
+
+assume val sid_hash : sid_t -> US.t
+
+open Pulse.Lib.Mutex
+
+// TODO: mark this as const for Rust extraction
+
 ```pulse
-fn alloc_global_state ()
+fn initialize_global_state ()
   requires emp
-  returns _:global_state_t
+  returns m:mutex global_state_mutex_pred
   ensures emp
 {
-  let sid_counter = R.alloc #sid_t 0ul;
-  let session_table_c = HT.alloc #sid_t #session_state sid_hash 256sz;
-  with stm. assert (models session_table_c stm);
-  let session_table = R.alloc session_table_c;
-  Pulse.Lib.OnRange.on_range_empty #emp_inames (session_perm stm) 0;
-  fold (global_state_lock_pred sid_counter session_table);
-  let lock = L.new_lock (global_state_lock_pred sid_counter session_table);
-  mk_global_state sid_counter session_table lock
+  let res = None #global_state_t;
+  rewrite emp as (global_state_mutex_pred res);
+  new_mutex global_state_mutex_pred res
 }
 ```
-let global_state : global_state_t = run_stt (alloc_global_state ())
+
+let global_state : mutex global_state_mutex_pred = run_stt (initialize_global_state ())
+
+#push-options "--ext 'pulse:env_on_err' --print_implicits --warn_error -342"
+```pulse
+fn alloc_global_state (r:ref (option global_state_t))
+  requires pts_to r None
+  ensures exists* gst. pts_to r (Some gst) ** global_state_mutex_pred (Some gst)
+{
+  let session_table = HT.alloc #sid_t #session_state sid_hash 256sz;
+  let st = {
+    session_id_counter = 0ul;
+    session_table;
+  };
+  with pht. assert (models session_table pht);
+  rewrite (models session_table pht) as (models st.session_table pht);
+  Pulse.Lib.OnRange.on_range_empty #emp_inames (session_perm pht) 0;
+  fold (global_state_mutex_pred (Some st));
+  r := Some st;
+}
+```
 
 (* Utilities to work with on_range (session_perm stm) *)
 (* <utilities on on_range> *)
-let session_table_eq_on_range  
+noextract  // TODO: why do we extract this at all, it is a prop
+let session_table_eq_on_range
   (stm0 stm1:session_table_map)
   (i j:nat)
-: prop
-= forall (k:sid_t). i <= U32.v k && U32.v k < j ==> PHT.lookup stm0 k == PHT.lookup stm1 k
+  : prop =
+  forall (k:sid_t). i <= U32.v k && U32.v k < j ==> PHT.lookup stm0 k == PHT.lookup stm1 k
 
 ```pulse
 ghost
@@ -213,117 +249,121 @@ fn frame_session_perm_on_range
 
 (* ----------- IMPLEMENTATION ----------- *)
 
-let coerce_us (x:pos_us) : SZ.t = x
+// let coerce_us (x:pos_us) : SZ.t = x
 
-(*
-  GetProfile: Part of DPE API 
-  Get the DPE's profile. 
-*)
+// (*
+//   GetProfile: Part of DPE API 
+//   Get the DPE's profile. 
+// *)
+// ```pulse
+// fn get_profile' ()
+//   requires emp
+//   returns d:profile_descriptor_t
+//   ensures emp
+// {
+//   mk_profile_descriptor
+//     (*name=*)""
+//     (*dpe_spec_version=*)1ul
+//     (*max_message_size=*)0ul // irrelevant: using direct interface
+//     (*uses_multi_part_messages=*)false
+//     (*supports_concurrent_operations=*)false // irrelevant by uses_multi_part_messages
+//     (*supports_encrypted_sessions=*)false // irrelevant by uses_multi_part_messages
+//     (*supports_derived_sessions=*)false // irrelevant by supports_encrypted_sessions
+//     (*max_sessions=*)0sz // irrelevant by supports_encrypted_sessions
+//     (*session_protocol=*)"" // irrelevant by supports_encrypted_sessions
+//     (*supports_session_sync=*)false // by supports_encrypted_sessions
+//     (*session_sync_policy=*)"" // irrelevant by supports_session_sync
+//     (*session_migration_protocol=*)"" // irrelevant by supports_session_migration
+//     (*supports_default_context=*)false
+//     (*supports_context_handles=*)true 
+//     (*max_contexts_per_session=*)1sz // 1 context per session
+//     (*max_context_handle_size=*)16sz // 16 bits
+//     (*supports_auto_init=*)false // irrelevant by supports_default_context
+//     (*supports_simulation=*)false
+//     (*supports_attestation=*)false
+//     (*supports_sealing=*)false 
+//     (*supports_get_profile=*)true
+//     (*supports_open_session=*)false // irrelevant by supports_encrypted_sessions
+//     (*supports_close_session=*)false // irrelevant by supports_encrypted_sessions
+//     (*supports_sync_session=*)false // irrelevant by supports_encrypted_sessions
+//     (*supports_export_session=*)false
+//     (*supports_import_session=*)false
+//     (*supports_init_context=*)true
+//     (*supports_certify_key=*)false // irrelevant by supports_attestation
+//     (*supports_sign=*)false // irrelevant by supports_attestation
+//     (*supports_seal=*)false // irrelevant by supports_sealing
+//     (*supports_unseal=*)false // irrelevant by supports_sealing
+//     (*supports_sealing_public=*)false // irrelevant by supports_sealing
+//     (*supports_rotate_context_handle=*)true
+//     (*dice_derivation=*)"" // FIXME: name for DICE algorithms
+//     (*asymmetric_derivation=*)"" // irrelevant by supports_attestation
+//     (*symmetric_derivation=*)"" // irrelevant by supports_attestation
+//     (*supports_any_label=*)false
+//     (*supported_labels=*)"" // FIXME: what are lables?
+//     (*initial_derivation=*)"" // FIXME: name?
+//     (*input_format=*)"" // FIXME: create CDDL spec for input record formats
+//     (*supports_internal_inputs=*)false
+//     (*supports_internal_dpe_info=*)false // irrelevant by supports_internal_inputs
+//     (*supports_internal_dpe_dice=*)false // irrelevant by supports_internal_inputs
+//     (*internal_dpe_info_type=*)"" // irrelevant by supports_internal_inputs
+//     (*internal_dpe_dice_type=*)"" // irrelevant by supports_internal_inputs
+//     (*internal_inputs=*)"" // irrelevant by supports_internal_inputs
+//     (*supports_certificates=*)false // irrelevant by supports_attestation
+//     (*max_certificate_size=*)0sz // irrelevant by supports_certificates
+//     (*max_certificate_chain_size=*)0sz // irrelevant by supports_certificates
+//     (*appends_more_certificates=*)false // irrelevant by supports_certificates
+//     (*supports_certificate_policies=*)false // irrelevant by supports_certificates
+//     (*supports_policy_identity_init=*)false // irrelevant by supports_certificate_policies
+//     (*supports_policy_identity_loc=*)false // irrelevant by supports_certificate_policies
+//     (*supports_policy_attest_init=*)false // irrelevant by supports_certificate_policies
+//     (*supports_policy_attest_loc=*)false // irrelevant by supports_certificate_policies
+//     (*supports_policy_assert_init=*)false // irrelevant by supports_certificate_policies
+//     (*supports_policy_assert_loc=*)false // irrelevant by supports_certificate_policies
+//     (*certificate_policies=*)"" // irrelevant by supports_certificate_policies
+//     (*supports_eca_certificates=*)false // irrelevant by supports_certificate_policies
+//     (*eca_certificate_format=*)"" // irrelevant by supports_eca_certificates
+//     (*leaf_certificate_format=*)"" // irrelevant by supports_certificates
+//     (*public_key_format=*)"" // irrelevant by supports_asymmetric_unseal
+//     (*supports_external_key=*)false // irrelevant by supports_certificates
+//     (*to_be_signed_format=*)"" // irrelevant by supports_sign
+//     (*signature_format=*)"" // irrelevant by supports_sign
+//     (*supports_symmetric_sign=*)false // irrelevant by supports_attestation
+//     (*supports_asymmetric_unseal=*)false // irrelevant by supports_attestation
+//     (*supports_unseal_policy=*)false// irrelevant by supports_sealing
+//     (*unseal_policy_format=*)"" // irrelevant by supports_unseal_policy 
+// }
+// ```
+// let get_profile = get_profile'
+
+
 ```pulse
-fn get_profile' ()
-  requires emp
-  returns d:profile_descriptor_t
-  ensures emp
-{
-  mk_profile_descriptor
-    (*name=*)""
-    (*dpe_spec_version=*)1ul
-    (*max_message_size=*)0ul // irrelevant: using direct interface
-    (*uses_multi_part_messages=*)false
-    (*supports_concurrent_operations=*)false // irrelevant by uses_multi_part_messages
-    (*supports_encrypted_sessions=*)false // irrelevant by uses_multi_part_messages
-    (*supports_derived_sessions=*)false // irrelevant by supports_encrypted_sessions
-    (*max_sessions=*)0sz // irrelevant by supports_encrypted_sessions
-    (*session_protocol=*)"" // irrelevant by supports_encrypted_sessions
-    (*supports_session_sync=*)false // by supports_encrypted_sessions
-    (*session_sync_policy=*)"" // irrelevant by supports_session_sync
-    (*session_migration_protocol=*)"" // irrelevant by supports_session_migration
-    (*supports_default_context=*)false
-    (*supports_context_handles=*)true 
-    (*max_contexts_per_session=*)1sz // 1 context per session
-    (*max_context_handle_size=*)16sz // 16 bits
-    (*supports_auto_init=*)false // irrelevant by supports_default_context
-    (*supports_simulation=*)false
-    (*supports_attestation=*)false
-    (*supports_sealing=*)false 
-    (*supports_get_profile=*)true
-    (*supports_open_session=*)false // irrelevant by supports_encrypted_sessions
-    (*supports_close_session=*)false // irrelevant by supports_encrypted_sessions
-    (*supports_sync_session=*)false // irrelevant by supports_encrypted_sessions
-    (*supports_export_session=*)false
-    (*supports_import_session=*)false
-    (*supports_init_context=*)true
-    (*supports_certify_key=*)false // irrelevant by supports_attestation
-    (*supports_sign=*)false // irrelevant by supports_attestation
-    (*supports_seal=*)false // irrelevant by supports_sealing
-    (*supports_unseal=*)false // irrelevant by supports_sealing
-    (*supports_sealing_public=*)false // irrelevant by supports_sealing
-    (*supports_rotate_context_handle=*)true
-    (*dice_derivation=*)"" // FIXME: name for DICE algorithms
-    (*asymmetric_derivation=*)"" // irrelevant by supports_attestation
-    (*symmetric_derivation=*)"" // irrelevant by supports_attestation
-    (*supports_any_label=*)false
-    (*supported_labels=*)"" // FIXME: what are lables?
-    (*initial_derivation=*)"" // FIXME: name?
-    (*input_format=*)"" // FIXME: create CDDL spec for input record formats
-    (*supports_internal_inputs=*)false
-    (*supports_internal_dpe_info=*)false // irrelevant by supports_internal_inputs
-    (*supports_internal_dpe_dice=*)false // irrelevant by supports_internal_inputs
-    (*internal_dpe_info_type=*)"" // irrelevant by supports_internal_inputs
-    (*internal_dpe_dice_type=*)"" // irrelevant by supports_internal_inputs
-    (*internal_inputs=*)"" // irrelevant by supports_internal_inputs
-    (*supports_certificates=*)false // irrelevant by supports_attestation
-    (*max_certificate_size=*)0sz // irrelevant by supports_certificates
-    (*max_certificate_chain_size=*)0sz // irrelevant by supports_certificates
-    (*appends_more_certificates=*)false // irrelevant by supports_certificates
-    (*supports_certificate_policies=*)false // irrelevant by supports_certificates
-    (*supports_policy_identity_init=*)false // irrelevant by supports_certificate_policies
-    (*supports_policy_identity_loc=*)false // irrelevant by supports_certificate_policies
-    (*supports_policy_attest_init=*)false // irrelevant by supports_certificate_policies
-    (*supports_policy_attest_loc=*)false // irrelevant by supports_certificate_policies
-    (*supports_policy_assert_init=*)false // irrelevant by supports_certificate_policies
-    (*supports_policy_assert_loc=*)false // irrelevant by supports_certificate_policies
-    (*certificate_policies=*)"" // irrelevant by supports_certificate_policies
-    (*supports_eca_certificates=*)false // irrelevant by supports_certificate_policies
-    (*eca_certificate_format=*)"" // irrelevant by supports_eca_certificates
-    (*leaf_certificate_format=*)"" // irrelevant by supports_certificates
-    (*public_key_format=*)"" // irrelevant by supports_asymmetric_unseal
-    (*supports_external_key=*)false // irrelevant by supports_certificates
-    (*to_be_signed_format=*)"" // irrelevant by supports_sign
-    (*signature_format=*)"" // irrelevant by supports_sign
-    (*supports_symmetric_sign=*)false // irrelevant by supports_attestation
-    (*supports_asymmetric_unseal=*)false // irrelevant by supports_attestation
-    (*supports_unseal_policy=*)false// irrelevant by supports_sealing
-    (*unseal_policy_format=*)"" // irrelevant by supports_unseal_policy 
-}
-```
-let get_profile = get_profile'
-
-
-```pulse
-fn insert (#kt:eqtype) (#vt:Type0)
-  (r:ref (ht_t kt vt)) (k:kt) (v:vt)
-  (#ht:erased (ht_t kt vt))
+fn insert_dpe (#kt:eqtype) (#vt:Type0)
+  (ht:ht_t kt vt) (k:kt) (v:vt)
   (#pht:erased (PHT.pht_t kt vt))
-  requires pts_to r ht ** models ht pht
-  returns b:bool
+  requires models ht pht
+  returns b:(ht_t kt vt & bool)
   ensures
     exists* pht'.
-      pts_to r ht **
-      models ht pht' **
-      pure (if b
+      models (fst b) pht' **
+      pure ((fst b).sz == ht.sz /\
+            (fst b).hashf == ht.hashf /\
+            (if snd b
             then (PHT.not_full (reveal pht).repr /\
                   pht'==PHT.insert pht k v)
-            else pht'==pht)
+            else pht'==pht))
 {
-  let b = not_full r;
-  if b
+  let b = not_full ht;
+  rewrite (models ht pht) as (models (fst b) pht);
+  if snd b
   {
-    Pulse.Lib.HashTable.insert r k v;
+    // rewrite (models ht pht) as (models (fst b) pht);
+    Pulse.Lib.HashTable.insert (fst b) k v
   }
   else
   {
-    false
+    let res = (fst b, false);
+    rewrite (models (fst b) pht) as (models (fst res) pht);
+    res
   }
 }
 ```
@@ -336,7 +376,7 @@ fn insert (#kt:eqtype) (#vt:Type0)
   NOTE: Current implementation disregards session protocol 
 *)
 ```pulse
-fn open_session' ()
+fn open_session ()
   requires emp
   returns _:option sid_t
   ensures emp
@@ -384,792 +424,792 @@ fn open_session' ()
   }
 }
 ```
-let open_session = open_session'
+// let open_session = open_session'
 
-assume val dbg : vprop
+// assume val dbg : vprop
 
-let uds_of_engine_context_repr (r:_{Engine_context_repr? r}) : erased (Seq.seq U8.t)=
-  match r with
-  | Engine_context_repr uds_bytes -> uds_bytes
+// let uds_of_engine_context_repr (r:_{Engine_context_repr? r}) : erased (Seq.seq U8.t)=
+//   match r with
+//   | Engine_context_repr uds_bytes -> uds_bytes
 
-
-```pulse 
-fn destroy_ctxt (ctxt:context_t) (#repr:erased context_repr_t)
-  requires context_perm ctxt repr
-  ensures emp
-{
-  match ctxt
-  {
-    Engine_context c ->
-    {
-      rewrite each ctxt as (Engine_context c);
-      let uds = get_engine_context_perm c repr;
-      unfold (engine_context_perm c uds);
-      A.zeroize uds_len c.uds;
-      A.free c.uds;
-    }
-    L0_context c ->
-    {
-      rewrite each ctxt as (L0_context c);
-      let r = get_l0_context_perm c repr;
-      unfold (l0_context_perm c r);
-      with s. assert (A.pts_to c.cdi s);
-      A.zeroize dice_digest_len c.cdi;
-      A.free c.cdi;
-    }
-    L1_context c ->
-    {
-      rewrite each ctxt as (L1_context c);
-      let r = get_l1_context_perm c repr;
-      unfold (l1_context_perm c r);
-      A.free c.deviceID_priv;
-      A.free c.deviceID_pub;
-      A.free c.aliasKey_priv;
-      A.free c.aliasKey_pub;
-      A.free c.aliasKeyCRT;
-      A.free c.deviceIDCSR;
-    }
-  }
-}
-```
-
-let opt #a (p:a -> vprop) (x:option a) : vprop =
-  match x with
-  | None -> emp
-  | Some x -> p x
-
-let available_session_state_perm (s:session_state) =
-  session_state_perm s ** pure (Available? s)
-
-```pulse
-fn return_none (a:Type0) (#p:(a -> vprop))
-  requires emp
-  returns o:option a
-  ensures opt p o
-{
-  rewrite emp as (opt p (None #a));
-  None #a
-}
-```
-
-let dflt #a (x:option a) (y:a) =
-  match x with
-  | Some v -> v
-  | _ -> y
-
-```pulse
-fn take_session_state (sid:sid_t) (replace:session_state)
-   requires session_state_perm replace
-   returns r:option session_state
-   ensures session_state_perm (dflt r replace)
-  {
-    L.acquire global_state.lock;
-    unfold (global_state_lock_pred global_state.session_id_counter global_state.session_table);
-    let max_sid = !global_state.session_id_counter;
-    if U32.(sid < max_sid)
-    {
-      with stm. assert (on_range (session_perm stm) 0 (U32.v max_sid));
-      with ht. assert (pts_to global_state.session_table ht);
-      assert (models ht stm);
-      let ss = HT.lookup global_state.session_table sid;
-      assert (models ht stm);
-      if fst ss
-      {
-        match snd ss 
-        {
-          Some st ->
-          {
-            let ok = insert global_state.session_table sid replace;
-            if ok
-            {
-              Pulse.Lib.OnRange.on_range_get #emp_inames (U32.v sid);
-              rewrite (session_perm stm (U32.v sid))
-                   as (session_state_perm st);
-              with stm'. assert (models ht stm');
-              frame_session_perm_on_range stm stm' 0 (U32.v sid);
-              // with stm0. assert (on_range (session_perm stm0) 
-              //                             (U32.v sid `Prims.op_Addition` 1)
-              //                             (U32.v max_sid));
-              frame_session_perm_on_range stm stm' (U32.v sid `Prims.op_Addition` 1) (U32.v max_sid);
-              rewrite (session_state_perm replace)
-                  as  (session_perm stm' (U32.v sid));
-              Pulse.Lib.OnRange.on_range_put #emp_inames 
-                    0 (U32.v sid) (U32.v max_sid)
-                    #(session_perm stm');
-              fold (global_state_lock_pred global_state.session_id_counter global_state.session_table);
-              L.release global_state.lock;
-              Some st
-            }
-            else
-            {
-              assert (models ht stm);
-              fold (global_state_lock_pred global_state.session_id_counter global_state.session_table);
-              L.release global_state.lock;
-              None #session_state
-              // return_none session_state #(session_state_perm)
-            }
-          }
-
-          None -> 
-          {
-            fold (global_state_lock_pred global_state.session_id_counter global_state.session_table);
-            L.release global_state.lock;
-            None #session_state
-            // return_none session_state #(session_state_perm)
-          }
-        }
-      }
-      else 
-      {
-        fold (global_state_lock_pred global_state.session_id_counter global_state.session_table);
-        L.release global_state.lock;
-        None #session_state
-        // return_none session_state #(session_state_perm)
-      }
-    }
-    else
-    {
-      fold (global_state_lock_pred global_state.session_id_counter global_state.session_table);
-      L.release global_state.lock;
-      None #session_state
-      // return_none session_state #(session_state_perm)
-    }
-  }
-  ```
 
 // ```pulse 
-// fn destroy_locked_ctxt (locked_ctxt:locked_context_t)
+// fn destroy_ctxt (ctxt:context_t) (#repr:erased context_repr_t)
+//   requires context_perm ctxt repr
+//   ensures emp
+// {
+//   match ctxt
+//   {
+//     Engine_context c ->
+//     {
+//       rewrite each ctxt as (Engine_context c);
+//       let uds = get_engine_context_perm c repr;
+//       unfold (engine_context_perm c uds);
+//       A.zeroize uds_len c.uds;
+//       A.free c.uds;
+//     }
+//     L0_context c ->
+//     {
+//       rewrite each ctxt as (L0_context c);
+//       let r = get_l0_context_perm c repr;
+//       unfold (l0_context_perm c r);
+//       with s. assert (A.pts_to c.cdi s);
+//       A.zeroize dice_digest_len c.cdi;
+//       A.free c.cdi;
+//     }
+//     L1_context c ->
+//     {
+//       rewrite each ctxt as (L1_context c);
+//       let r = get_l1_context_perm c repr;
+//       unfold (l1_context_perm c r);
+//       A.free c.deviceID_priv;
+//       A.free c.deviceID_pub;
+//       A.free c.aliasKey_priv;
+//       A.free c.aliasKey_pub;
+//       A.free c.aliasKeyCRT;
+//       A.free c.deviceIDCSR;
+//     }
+//   }
+// }
+// ```
+
+// let opt #a (p:a -> vprop) (x:option a) : vprop =
+//   match x with
+//   | None -> emp
+//   | Some x -> p x
+
+// let available_session_state_perm (s:session_state) =
+//   session_state_perm s ** pure (Available? s)
+
+// ```pulse
+// fn return_none (a:Type0) (#p:(a -> vprop))
+//   requires emp
+//   returns o:option a
+//   ensures opt p o
+// {
+//   rewrite emp as (opt p (None #a));
+//   None #a
+// }
+// ```
+
+// let dflt #a (x:option a) (y:a) =
+//   match x with
+//   | Some v -> v
+//   | _ -> y
+
+// ```pulse
+// fn take_session_state (sid:sid_t) (replace:session_state)
+//    requires session_state_perm replace
+//    returns r:option session_state
+//    ensures session_state_perm (dflt r replace)
+//   {
+//     L.acquire global_state.lock;
+//     unfold (global_state_lock_pred global_state.session_id_counter global_state.session_table);
+//     let max_sid = !global_state.session_id_counter;
+//     if U32.(sid < max_sid)
+//     {
+//       with stm. assert (on_range (session_perm stm) 0 (U32.v max_sid));
+//       with ht. assert (pts_to global_state.session_table ht);
+//       assert (models ht stm);
+//       let ss = HT.lookup global_state.session_table sid;
+//       assert (models ht stm);
+//       if fst ss
+//       {
+//         match snd ss 
+//         {
+//           Some st ->
+//           {
+//             let ok = insert global_state.session_table sid replace;
+//             if ok
+//             {
+//               Pulse.Lib.OnRange.on_range_get #emp_inames (U32.v sid);
+//               rewrite (session_perm stm (U32.v sid))
+//                    as (session_state_perm st);
+//               with stm'. assert (models ht stm');
+//               frame_session_perm_on_range stm stm' 0 (U32.v sid);
+//               // with stm0. assert (on_range (session_perm stm0) 
+//               //                             (U32.v sid `Prims.op_Addition` 1)
+//               //                             (U32.v max_sid));
+//               frame_session_perm_on_range stm stm' (U32.v sid `Prims.op_Addition` 1) (U32.v max_sid);
+//               rewrite (session_state_perm replace)
+//                   as  (session_perm stm' (U32.v sid));
+//               Pulse.Lib.OnRange.on_range_put #emp_inames 
+//                     0 (U32.v sid) (U32.v max_sid)
+//                     #(session_perm stm');
+//               fold (global_state_lock_pred global_state.session_id_counter global_state.session_table);
+//               L.release global_state.lock;
+//               Some st
+//             }
+//             else
+//             {
+//               assert (models ht stm);
+//               fold (global_state_lock_pred global_state.session_id_counter global_state.session_table);
+//               L.release global_state.lock;
+//               None #session_state
+//               // return_none session_state #(session_state_perm)
+//             }
+//           }
+
+//           None -> 
+//           {
+//             fold (global_state_lock_pred global_state.session_id_counter global_state.session_table);
+//             L.release global_state.lock;
+//             None #session_state
+//             // return_none session_state #(session_state_perm)
+//           }
+//         }
+//       }
+//       else 
+//       {
+//         fold (global_state_lock_pred global_state.session_id_counter global_state.session_table);
+//         L.release global_state.lock;
+//         None #session_state
+//         // return_none session_state #(session_state_perm)
+//       }
+//     }
+//     else
+//     {
+//       fold (global_state_lock_pred global_state.session_id_counter global_state.session_table);
+//       L.release global_state.lock;
+//       None #session_state
+//       // return_none session_state #(session_state_perm)
+//     }
+//   }
+//   ```
+
+// // ```pulse 
+// // fn destroy_locked_ctxt (locked_ctxt:locked_context_t)
+// //   requires emp
+// //   ensures emp
+// // {
+// //   let ctxt = locked_ctxt._1;
+// //   let repr = locked_ctxt._2;
+// //   let ctxt_lk = locked_ctxt._3;
+// //   // TODO: would be nice to use a rename here, to transfer ownership to ctxt_lk
+// //   L.acquire locked_ctxt._3;
+// //   destroy_ctxt locked_ctxt._1;
+// // }
+// // ```
+
+
+
+// (*
+//   DestroyContext: Part of DPE API 
+//   Destroy the context pointed to by the handle by freeing the
+//   arrays in the context (zeroize the UDS, if applicable). Return
+//   boolean indicating success. 
+//   NOTE: Current implementation disregards session protocol 
+// *)
+// ```pulse
+// fn destroy_context' (sid:sid_t) (ctxt_hndl:ctxt_hndl_t)
+//   requires emp
+//   returns b:bool
+//   ensures emp
+// {
+//   rewrite emp as (session_state_perm InUse);
+//   let st = take_session_state sid InUse;
+//   match st
+//   {
+//     None ->
+//     {
+//       with s. rewrite (session_state_perm s) as emp;
+//       false
+//     }
+
+//     Some st ->
+//     {
+//       with s. rewrite (session_state_perm s)
+//                    as (session_state_perm st);
+//       if not (Available? st)
+//       {
+//         rewrite (session_state_perm st) as emp;
+//         rewrite emp as (session_state_perm SessionError);
+//         let st' = take_session_state sid SessionError;
+//         //TODO: Fix this by proving that st' must be present and InUse
+//         drop_ (session_state_perm (dflt st' SessionError));
+//         false
+//       }
+//       else if (ctxt_hndl = hndl_of st)
+//       {
+//         elim_session_state_perm_available st;
+//         destroy_ctxt (ctxt_of st);
+//         //reset the session to the start state
+//         rewrite emp as (session_state_perm SessionStart);
+//         let st' = take_session_state sid SessionStart;
+//         //TODO: Fix this by proving that st' must be present and InUse
+//         drop_ (session_state_perm (dflt st' SessionStart));
+//         true
+//       }
+//       else
+//       {
+//         //context handle mismatch; put back st
+//         //and return false
+//         let st' = take_session_state sid st;
+//         //TODO: Fix this by proving that st' must be present and InUse
+//         drop_ (session_state_perm (dflt st' st));
+//         false
+//       }
+//     }
+//   }
+// }
+// ```
+
+// let destroy_context = destroy_context'
+
+// ```pulse
+// fn ctxt_hndl_do_nothing (k:ctxt_hndl_t)
 //   requires emp
 //   ensures emp
 // {
-//   let ctxt = locked_ctxt._1;
-//   let repr = locked_ctxt._2;
-//   let ctxt_lk = locked_ctxt._3;
-//   // TODO: would be nice to use a rename here, to transfer ownership to ctxt_lk
-//   L.acquire locked_ctxt._3;
-//   destroy_ctxt locked_ctxt._1;
+//   ()
+// }
+// ```
+
+// ```pulse
+// fn destroy_session_state (st:session_state)
+//   requires session_state_perm st
+//   ensures emp
+// {
+//   if not (Available? st)
+//   {
+//     rewrite (session_state_perm st) as emp
+//   }
+//   else 
+//   {
+//     elim_session_state_perm_available st;
+//     destroy_ctxt (ctxt_of st);
+//   }
+// }
+// ```
+
+// (* 
+//   CloseSession: Part of DPE API 
+//   Destroy the context table for the session and remove the reference
+//   to it from the session table. Return boolean indicating success. 
+//   NOTE: Current implementation disregards session protocol 
+// *)
+// ```pulse
+// fn close_session' (sid:sid_t)
+//   requires emp
+//   returns b:bool
+//   ensures emp
+// {
+//   rewrite emp as (session_state_perm InUse);
+//   let st = take_session_state sid InUse;
+//   match st 
+//   {
+//     None -> 
+//     {
+//       with s. rewrite (session_state_perm s) as emp;
+//       false 
+//     }
+
+//     Some st ->
+//     {
+//       destroy_session_state st;
+//       rewrite emp as (session_state_perm SessionClosed);
+//       let st' = take_session_state sid SessionClosed;
+//       //TODO: Fix this by proving that st' must be present and InUse
+//       drop_ (session_state_perm (dflt st' SessionClosed));
+//       true
+//     }
+//   }
+// }
+// ```
+// let close_session = close_session'
+
+// // TODO: 
+// let prng () : U32.t = admit()
+
+// ```pulse
+// fn init_engine_ctxt (uds:A.larray U8.t (US.v uds_len))
+//                     (#p:perm)
+//                     (#uds_bytes:Ghost.erased (Seq.seq U8.t))
+//   requires A.pts_to uds #p uds_bytes
+//   returns ctxt:context_t
+//   ensures A.pts_to uds #p uds_bytes **
+//           context_perm ctxt (Engine_context_repr uds_bytes)
+// { 
+//   let uds_buf = A.alloc 0uy uds_len;
+//   memcpy uds_len uds uds_buf;
+//   let engine_context = mk_engine_context_t uds_buf;
+
+//   rewrite each uds_buf as (engine_context.uds);
+//   fold (engine_context_perm engine_context uds_bytes);
+
+//   let ctxt = mk_context_t_engine engine_context;
+//   rewrite (engine_context_perm engine_context uds_bytes) 
+//     as (context_perm ctxt (Engine_context_repr uds_bytes));
+//   ctxt
+// }
+// ```
+
+// ```pulse
+// fn init_l0_ctxt (cdi:A.larray U8.t (US.v dice_digest_len))  
+//                 (#engine_repr:erased engine_record_repr)
+//                 (#s:erased (Seq.seq U8.t))
+//                 (#uds_bytes:erased (Seq.seq U8.t))
+//                 (_:squash(cdi_functional_correctness s uds_bytes engine_repr
+//                       /\ l0_is_authentic engine_repr))
+//   requires A.pts_to cdi s
+//         ** pure (A.is_full_array cdi)
+//   returns ctxt:context_t
+//   ensures exists* repr.
+//     context_perm ctxt repr **
+//     pure (repr == L0_context_repr (mk_l0_context_repr_t uds_bytes s engine_repr))
+// {
+//   let cdi_buf = A.alloc 0uy dice_digest_len;
+//   memcpy dice_digest_len cdi cdi_buf;
+//   A.zeroize dice_digest_len cdi;
+//   A.free cdi;
+
+//   let l0_context = mk_l0_context_t cdi_buf;
+//   let l0_context_repr = hide (mk_l0_context_repr_t uds_bytes s engine_repr);
+//   rewrite each cdi_buf as (l0_context.cdi);
+//   fold (l0_context_perm l0_context l0_context_repr);
+
+//   let ctxt = mk_context_t_l0 l0_context;
+//   let repr = mk_context_repr_t_l0 l0_context_repr;
+//   rewrite (l0_context_perm l0_context l0_context_repr) 
+//     as (context_perm ctxt repr);
+
+//   ctxt
+// }
+// ```
+
+// ```pulse
+// fn init_l1_ctxt (deviceIDCSR_len: US.t) (aliasKeyCRT_len: US.t) 
+//                 (deviceID_priv: A.larray U8.t (US.v v32us)) (deviceID_pub: A.larray U8.t (US.v v32us))
+//                 (aliasKey_priv: A.larray U8.t (US.v v32us)) (aliasKey_pub: A.larray U8.t (US.v v32us)) 
+//                 (deviceIDCSR: A.larray U8.t (US.v deviceIDCSR_len)) (aliasKeyCRT: A.larray U8.t (US.v aliasKeyCRT_len))
+//                 (deviceID_label_len aliasKey_label_len: erased hkdf_lbl_len)
+//                 (cdi:erased (Seq.seq U8.t))
+//                 (repr:erased l0_record_repr_t)
+//                 (deviceIDCSR_ingredients:erased deviceIDCSR_ingredients_t)
+//                 (aliasKeyCRT_ingredients:erased aliasKeyCRT_ingredients_t)
+//                 (#deviceID_priv0 #deviceID_pub0 #aliasKey_priv0 #aliasKey_pub0
+//                  #deviceIDCSR0 #aliasKeyCRT0:erased (Seq.seq U8.t))
+              
+//   requires A.pts_to deviceID_priv deviceID_priv0 ** 
+//            A.pts_to deviceID_pub deviceID_pub0 ** 
+//            A.pts_to aliasKey_priv aliasKey_priv0 ** 
+//            A.pts_to aliasKey_pub aliasKey_pub0 ** 
+//            A.pts_to deviceIDCSR deviceIDCSR0 **
+//            A.pts_to aliasKeyCRT aliasKeyCRT0 **
+//            pure (
+//             valid_hkdf_ikm_len dice_digest_len
+//                        /\ aliasKey_functional_correctness
+//                             dice_hash_alg dice_digest_len cdi repr.fwid
+//                             aliasKey_label_len repr.aliasKey_label 
+//                             aliasKey_pub0 aliasKey_priv0
+//                        /\ deviceIDCSR_functional_correctness 
+//                             dice_hash_alg dice_digest_len cdi
+//                             deviceID_label_len repr.deviceID_label deviceIDCSR_ingredients 
+//                             deviceIDCSR_len deviceIDCSR0 
+//                        /\ aliasKeyCRT_functional_correctness 
+//                             dice_hash_alg dice_digest_len cdi repr.fwid
+//                             deviceID_label_len repr.deviceID_label aliasKeyCRT_ingredients 
+//                             aliasKeyCRT_len aliasKeyCRT0 aliasKey_pub0
+//            )
+//   returns ctxt:context_t
+//   ensures 
+//     A.pts_to deviceID_priv deviceID_priv0 ** 
+//     A.pts_to deviceID_pub deviceID_pub0 **
+//     A.pts_to aliasKey_priv aliasKey_priv0 ** 
+//     A.pts_to aliasKey_pub aliasKey_pub0 ** 
+//     A.pts_to deviceIDCSR deviceIDCSR0 **
+//     A.pts_to aliasKeyCRT aliasKeyCRT0 **
+//     (exists* l1repr. 
+//       context_perm ctxt l1repr **
+//       pure (l1repr ==
+//             L1_context_repr (mk_l1_context_repr_t 
+//                               deviceID_label_len aliasKey_label_len deviceID_priv0 deviceID_pub0
+//                               aliasKey_priv0 aliasKey_pub0 aliasKeyCRT_len aliasKeyCRT0 deviceIDCSR_len
+//                               deviceIDCSR0 cdi repr deviceIDCSR_ingredients aliasKeyCRT_ingredients))
+//     )
+
+// {
+//   let deviceID_pub_buf = A.alloc 0uy v32us;
+//   let deviceID_priv_buf = A.alloc 0uy v32us;
+//   let aliasKey_priv_buf = A.alloc 0uy v32us;
+//   let aliasKey_pub_buf = A.alloc 0uy v32us;
+//   let deviceIDCSR_buf = A.alloc 0uy deviceIDCSR_len;
+//   let aliasKeyCRT_buf = A.alloc 0uy aliasKeyCRT_len;
+//   memcpy v32us deviceID_priv deviceID_priv_buf;
+//   memcpy v32us deviceID_pub deviceID_pub_buf;
+//   memcpy v32us aliasKey_priv aliasKey_priv_buf;
+//   memcpy v32us aliasKey_pub aliasKey_pub_buf;
+//   memcpy deviceIDCSR_len deviceIDCSR deviceIDCSR_buf;
+//   memcpy aliasKeyCRT_len aliasKeyCRT aliasKeyCRT_buf;
+
+//   let l1_context = mk_l1_context_t 
+//     deviceID_priv_buf deviceID_pub_buf aliasKey_priv_buf aliasKey_pub_buf 
+//     aliasKeyCRT_buf deviceIDCSR_buf;
+//   let l1_context_repr = hide (mk_l1_context_repr_t 
+//     deviceID_label_len aliasKey_label_len deviceID_priv0 deviceID_pub0
+//     aliasKey_priv0 aliasKey_pub0 aliasKeyCRT_len aliasKeyCRT0 deviceIDCSR_len
+//     deviceIDCSR0 cdi repr deviceIDCSR_ingredients aliasKeyCRT_ingredients);
+
+//   rewrite each deviceID_priv_buf  as l1_context.deviceID_priv,
+//           deviceID_pub_buf  as l1_context.deviceID_pub,
+//           aliasKey_priv_buf as l1_context.aliasKey_priv,
+//           aliasKey_pub_buf  as l1_context.aliasKey_pub,
+//           deviceIDCSR_buf   as l1_context.deviceIDCSR,
+//           aliasKeyCRT_buf   as l1_context.aliasKeyCRT;
+
+//   fold (l1_context_perm l1_context l1_context_repr);
+
+//   let ctxt = mk_context_t_l1 l1_context;
+//   let repr = mk_context_repr_t_l1 l1_context_repr;
+//   rewrite (l1_context_perm l1_context l1_context_repr) as (context_perm ctxt repr);
+//   ctxt  
+// }
+// ```
+
+// (*
+//   InitializeContext: Part of DPE API 
+//   Create a context in the initial state (engine context) and store the context
+//   in the current session's context table. Return the context handle upon
+//   success and None upon failure. 
+// *)
+// ```pulse
+// fn initialize_context'
+//   (#p:perm) (#uds_bytes:Ghost.erased (Seq.seq U8.t))
+//   (sid:sid_t) (uds:A.larray U8.t (US.v uds_len)) 
+                       
+//   requires A.pts_to uds #p uds_bytes
+//   returns _:option ctxt_hndl_t
+//   ensures A.pts_to uds #p uds_bytes
+// {
+//   rewrite emp as (session_state_perm InUse);
+//   let st = take_session_state sid InUse;
+//   match st 
+//   {
+//     None ->
+//     {
+//       with s. rewrite (session_state_perm s) as emp;
+//       None #ctxt_hndl_t
+//     }
+    
+//     Some st ->
+//     {
+//       if SessionStart? st 
+//       {
+//         rewrite (session_state_perm st) as emp;
+//         let ctxt = init_engine_ctxt uds;
+//         let ctxt_hndl = prng ();
+//         let st' = intro_session_state_perm_available ctxt ctxt_hndl;
+//         let st'' = take_session_state sid st';
+//         //TODO: prove that st'' is InUse
+//         drop_ (session_state_perm (dflt st'' st'));
+//         Some ctxt_hndl
+//       }
+//       else //session error
+//       {
+//         destroy_session_state st;
+//         rewrite emp as (session_state_perm SessionError);
+//         let st' = take_session_state sid SessionError;
+//         //TODO: prove st' is InUse
+//         drop_ (session_state_perm (dflt st' SessionError));
+//         None #ctxt_hndl_t
+//       }
+//     }
+//   }
+// }
+// ```
+
+// let initialize_context = initialize_context'
+
+// (*
+//   RotateContextHandle: Part of DPE API 
+//   Invalidate the current context handle and replace it with a new context
+//   handle. Return the context handle upon success and None upon failure.
+// *)
+// ```pulse
+// fn rotate_context_handle' (sid:sid_t) (ctxt_hndl:ctxt_hndl_t)
+//   requires emp
+//   returns _:option ctxt_hndl_t
+//   ensures emp
+// {
+//   rewrite emp as (session_state_perm InUse);
+//   let st = take_session_state sid InUse;
+//   match st 
+//   {
+//     None ->
+//     {
+//       with s. rewrite (session_state_perm s) as emp;
+//       None #ctxt_hndl_t
+//     }
+
+//     Some st ->
+//     {
+//       if InUse? st
+//       { //block concurrent access
+//         rewrite (session_state_perm st) as emp;
+//         None #ctxt_hndl_t
+//       }
+//       else if not (Available? st)
+//       { //session error
+//         rewrite (session_state_perm st) as emp;
+//         rewrite emp as (session_state_perm SessionError);
+//         let st' = take_session_state sid SessionError;
+//         //TODO: prove st' is InUse
+//         drop_ (session_state_perm (dflt st' SessionError));
+//         None #ctxt_hndl_t
+//       }
+//       else 
+//       {
+//         let new_ctxt_hndl = prng ();
+//         elim_session_state_perm_available st;
+//         let st' = intro_session_state_perm_available (ctxt_of st) new_ctxt_hndl;
+//         let st'' = take_session_state sid st';
+//         //TODO: prove st'' is InUse
+//         drop_ (session_state_perm (dflt st'' st'));
+//         Some new_ctxt_hndl
+//       }      
+//     }
+//   }
+// }
+// ```
+// let rotate_context_handle = rotate_context_handle'
+
+// let maybe_context_perm (o:option context_t) =
+//   match o with
+//   | None -> emp
+//   | _ -> exists* repr. context_perm (Some?.v o) repr
+
+// ```pulse
+// fn intro_maybe_context_perm (c:context_t)
+//   requires context_perm c 'repr
+//   returns o:option context_t
+//   ensures maybe_context_perm o
+// {
+//   rewrite (context_perm c 'repr)
+//        as (context_perm (Some?.v (Some c)) 'repr);
+//   fold (maybe_context_perm (Some c));
+//   Some c
+// }
+// ```
+
+// ```pulse
+// ghost
+// fn elim_maybe_context_perm (c:context_t)
+//   requires maybe_context_perm (Some c)
+//   ensures exists* repr. context_perm c repr
+// {
+//   unfold (maybe_context_perm (Some c));
+//   with x y. rewrite (context_perm x y) as (context_perm c y)
+// }
+// ```
+
+// ```pulse
+// fn derive_child_from_context
+//     (context:context_t)
+//     (record:record_t)
+//   requires
+//     record_perm record p 'record_repr **
+//     context_perm context 'context_repr
+//   returns res:option context_t
+//   ensures
+//     record_perm record p 'record_repr **
+//     context_perm context 'context_repr **
+//     maybe_context_perm res
+// {
+//   match context
+//   {
+//     Engine_context c ->
+//     {
+//       if not (Engine_record? record)
+//       { //illegal argument; reject
+//         rewrite emp as (maybe_context_perm None);
+//         None #context_t
+//       }
+//       else
+//       {
+//         rewrite each context as (Engine_context c);
+//         let uds = get_engine_context_perm c 'context_repr;
+//         // rewrite (context_perm (E) ctxt_repr) as (engine_context_perm c);
+//         unfold (engine_context_perm c uds);
+//         match record
+//         {
+//           Engine_record r ->
+//           {
+//             rewrite each record as (Engine_record r);
+//             let r0 = get_engine_record_perm r 'record_repr p;
+//             let cdi = A.alloc 0uy dice_digest_len;
+//             let ret = EngineCore.engine_main cdi c.uds r;
+//             with s. assert (A.pts_to cdi s);
+//             fold (engine_context_perm c uds);
+//             rewrite (engine_context_perm c uds)
+//                  as (context_perm context 'context_repr);
+//             match ret 
+//             {
+//               DICE_SUCCESS ->
+//               {
+//                 let l0_ctxt = init_l0_ctxt cdi #r0 #s #uds ();
+//                 rewrite (engine_record_perm r p r0)
+//                      as (record_perm record p 'record_repr);
+//                 let l0_ctxt_opt = intro_maybe_context_perm l0_ctxt;
+//                 l0_ctxt_opt
+//               }
+
+//               DICE_ERROR ->
+//               {
+//                 A.zeroize dice_digest_len cdi;
+//                 A.free cdi;
+//                 rewrite (engine_record_perm r p r0)
+//                      as (record_perm record p 'record_repr);
+//                 rewrite emp as (maybe_context_perm None);
+//                 None #context_t
+//               }
+//             }
+//           }
+//         }
+//       }
+//     }
+//     L0_context c ->
+//     { 
+//       if not (L0_record? record)
+//       { //illegal argument; reject
+//         rewrite emp as (maybe_context_perm None);
+//         None #context_t
+//       }
+//       else
+//       {
+//         match record 
+//         {
+//           L0_record r ->
+//           {
+//             // NOTE: we won't eventually release l0_context_perm because we won't 
+//             // own it anymore -- we will free the cdi array
+//             rewrite each context as (L0_context c);
+//             let cr = get_l0_context_perm c 'context_repr;
+//             unfold (l0_context_perm c cr);
+//             with s. assert (A.pts_to c.cdi s);
+
+//             rewrite each record as (L0_record r);
+//             let r0 = get_l0_record_perm r 'record_repr p;
+
+//             let idcsr_ing = r.deviceIDCSR_ingredients;
+//             let akcrt_ing = r.aliasKeyCRT_ingredients;
+
+//             let deviceIDCRI_len = len_of_deviceIDCRI  idcsr_ing.version idcsr_ing.s_common 
+//                                                       idcsr_ing.s_org idcsr_ing.s_country;
+//             let aliasKeyTBS_len = len_of_aliasKeyTBS  akcrt_ing.serialNumber akcrt_ing.i_common 
+//                                                       akcrt_ing.i_org akcrt_ing.i_country 
+//                                                       akcrt_ing.s_common akcrt_ing.s_org 
+//                                                       akcrt_ing.s_country akcrt_ing.l0_version;
+//             let deviceIDCSR_len = length_of_deviceIDCSR deviceIDCRI_len;
+//             let aliasKeyCRT_len = length_of_aliasKeyCRT aliasKeyTBS_len;
+
+//             let mut deviceID_pub = [| 0uy; v32us |];
+//             let mut deviceID_priv = [| 0uy; v32us |];
+//             let mut aliasKey_pub = [| 0uy; v32us |];
+//             let mut aliasKey_priv = [| 0uy; v32us |];
+//             let mut deviceIDCSR = [| 0uy; deviceIDCSR_len |];
+//             let mut aliasKeyCRT = [| 0uy; aliasKeyCRT_len |];
+            
+//             L0Core.l0_main  c.cdi deviceID_pub deviceID_priv 
+//                             aliasKey_pub aliasKey_priv 
+//                             aliasKeyTBS_len aliasKeyCRT_len aliasKeyCRT 
+//                             deviceIDCRI_len deviceIDCSR_len deviceIDCSR r;
+//             fold (l0_context_perm c cr);
+//             rewrite (l0_context_perm c cr)
+//                  as (context_perm context 'context_repr);
+//             rewrite (l0_record_perm r p r0)
+//                  as (record_perm record p 'record_repr);
+//             let l1_context = init_l1_ctxt 
+//                         deviceIDCSR_len aliasKeyCRT_len deviceID_priv deviceID_pub
+//                         aliasKey_priv aliasKey_pub deviceIDCSR aliasKeyCRT
+//                         (hide r.deviceID_label_len)
+//                         (hide r.aliasKey_label_len) s r0 (hide idcsr_ing) (hide akcrt_ing);
+//             intro_maybe_context_perm l1_context
+//           }
+//         }
+//       }
+//     }
+//     L1_context _ ->
+//     {
+//       // ERROR - cannot invoke DeriveChild with L1 context
+//       rewrite emp as (maybe_context_perm None);
+//       None #context_t
+//     }
+//   }
 // }
 // ```
 
 
+// (*
+//   DeriveChild: Part of DPE API 
+//   Execute the DICE layer associated with the current context and produce a 
+//   new context. Destroy the current context in the current session's context table 
+//   and store the new context in the table. Return the new context handle upon
+//   success and None upon failure. 
+// *)
+// ```pulse
+// fn derive_child' (sid:sid_t) (ctxt_hndl:ctxt_hndl_t) (record:record_t)
+//                  (#repr:erased repr_t) (#p:perm)
+//   requires record_perm record p repr
+//   returns _:option ctxt_hndl_t
+//   ensures record_perm record p repr
+// {
+//   rewrite emp as (session_state_perm InUse);
+//   let st = take_session_state sid InUse;
+//   match st 
+//   {
+//     None ->
+//     {
+//       with s. rewrite (session_state_perm s) as emp;
+//       None #ctxt_hndl_t
+//     }
 
-(*
-  DestroyContext: Part of DPE API 
-  Destroy the context pointed to by the handle by freeing the
-  arrays in the context (zeroize the UDS, if applicable). Return
-  boolean indicating success. 
-  NOTE: Current implementation disregards session protocol 
-*)
-```pulse
-fn destroy_context' (sid:sid_t) (ctxt_hndl:ctxt_hndl_t)
-  requires emp
-  returns b:bool
-  ensures emp
-{
-  rewrite emp as (session_state_perm InUse);
-  let st = take_session_state sid InUse;
-  match st
-  {
-    None ->
-    {
-      with s. rewrite (session_state_perm s) as emp;
-      false
-    }
+//     Some st ->
+//     {
+//       if InUse? st
+//       { //block concurrent access
+//         rewrite (session_state_perm st) as emp;
+//         None #ctxt_hndl_t
+//       }
+//       else if not (Available? st)
+//       { //session error
+//         rewrite (session_state_perm st) as emp;
+//         rewrite emp as (session_state_perm SessionError);
+//         let st' = take_session_state sid SessionError;
+//         //TODO: prove st' is InUse
+//         drop_ (session_state_perm (dflt st' SessionError));
+//         None #ctxt_hndl_t
+//       }
+//       else 
+//       {
+//         elim_session_state_perm_available st;
+//         let next_ctxt = derive_child_from_context (ctxt_of st) record;
+//         destroy_ctxt (ctxt_of st);
+//         match next_ctxt
+//         {
+//           None ->
+//           {
+//             rewrite emp as (session_state_perm SessionError);
+//             rewrite (maybe_context_perm next_ctxt) as emp;
+//             let st' = take_session_state sid SessionError;
+//             //TODO: prove st' is InUse
+//             drop_ (session_state_perm (dflt st' SessionError));
+//             None #ctxt_hndl_t
+//           }
 
-    Some st ->
-    {
-      with s. rewrite (session_state_perm s)
-                   as (session_state_perm st);
-      if not (Available? st)
-      {
-        rewrite (session_state_perm st) as emp;
-        rewrite emp as (session_state_perm SessionError);
-        let st' = take_session_state sid SessionError;
-        //TODO: Fix this by proving that st' must be present and InUse
-        drop_ (session_state_perm (dflt st' SessionError));
-        false
-      }
-      else if (ctxt_hndl = hndl_of st)
-      {
-        elim_session_state_perm_available st;
-        destroy_ctxt (ctxt_of st);
-        //reset the session to the start state
-        rewrite emp as (session_state_perm SessionStart);
-        let st' = take_session_state sid SessionStart;
-        //TODO: Fix this by proving that st' must be present and InUse
-        drop_ (session_state_perm (dflt st' SessionStart));
-        true
-      }
-      else
-      {
-        //context handle mismatch; put back st
-        //and return false
-        let st' = take_session_state sid st;
-        //TODO: Fix this by proving that st' must be present and InUse
-        drop_ (session_state_perm (dflt st' st));
-        false
-      }
-    }
-  }
-}
-```
-
-let destroy_context = destroy_context'
-
-```pulse
-fn ctxt_hndl_do_nothing (k:ctxt_hndl_t)
-  requires emp
-  ensures emp
-{
-  ()
-}
-```
-
-```pulse
-fn destroy_session_state (st:session_state)
-  requires session_state_perm st
-  ensures emp
-{
-  if not (Available? st)
-  {
-    rewrite (session_state_perm st) as emp
-  }
-  else 
-  {
-    elim_session_state_perm_available st;
-    destroy_ctxt (ctxt_of st);
-  }
-}
-```
-
-(* 
-  CloseSession: Part of DPE API 
-  Destroy the context table for the session and remove the reference
-  to it from the session table. Return boolean indicating success. 
-  NOTE: Current implementation disregards session protocol 
-*)
-```pulse
-fn close_session' (sid:sid_t)
-  requires emp
-  returns b:bool
-  ensures emp
-{
-  rewrite emp as (session_state_perm InUse);
-  let st = take_session_state sid InUse;
-  match st 
-  {
-    None -> 
-    {
-      with s. rewrite (session_state_perm s) as emp;
-      false 
-    }
-
-    Some st ->
-    {
-      destroy_session_state st;
-      rewrite emp as (session_state_perm SessionClosed);
-      let st' = take_session_state sid SessionClosed;
-      //TODO: Fix this by proving that st' must be present and InUse
-      drop_ (session_state_perm (dflt st' SessionClosed));
-      true
-    }
-  }
-}
-```
-let close_session = close_session'
-
-// TODO: 
-let prng () : U32.t = admit()
-
-```pulse
-fn init_engine_ctxt (uds:A.larray U8.t (US.v uds_len))
-                    (#p:perm)
-                    (#uds_bytes:Ghost.erased (Seq.seq U8.t))
-  requires A.pts_to uds #p uds_bytes
-  returns ctxt:context_t
-  ensures A.pts_to uds #p uds_bytes **
-          context_perm ctxt (Engine_context_repr uds_bytes)
-{ 
-  let uds_buf = A.alloc 0uy uds_len;
-  memcpy uds_len uds uds_buf;
-  let engine_context = mk_engine_context_t uds_buf;
-
-  rewrite each uds_buf as (engine_context.uds);
-  fold (engine_context_perm engine_context uds_bytes);
-
-  let ctxt = mk_context_t_engine engine_context;
-  rewrite (engine_context_perm engine_context uds_bytes) 
-    as (context_perm ctxt (Engine_context_repr uds_bytes));
-  ctxt
-}
-```
-
-```pulse
-fn init_l0_ctxt (cdi:A.larray U8.t (US.v dice_digest_len))  
-                (#engine_repr:erased engine_record_repr)
-                (#s:erased (Seq.seq U8.t))
-                (#uds_bytes:erased (Seq.seq U8.t))
-                (_:squash(cdi_functional_correctness s uds_bytes engine_repr
-                      /\ l0_is_authentic engine_repr))
-  requires A.pts_to cdi s
-        ** pure (A.is_full_array cdi)
-  returns ctxt:context_t
-  ensures exists* repr.
-    context_perm ctxt repr **
-    pure (repr == L0_context_repr (mk_l0_context_repr_t uds_bytes s engine_repr))
-{
-  let cdi_buf = A.alloc 0uy dice_digest_len;
-  memcpy dice_digest_len cdi cdi_buf;
-  A.zeroize dice_digest_len cdi;
-  A.free cdi;
-
-  let l0_context = mk_l0_context_t cdi_buf;
-  let l0_context_repr = hide (mk_l0_context_repr_t uds_bytes s engine_repr);
-  rewrite each cdi_buf as (l0_context.cdi);
-  fold (l0_context_perm l0_context l0_context_repr);
-
-  let ctxt = mk_context_t_l0 l0_context;
-  let repr = mk_context_repr_t_l0 l0_context_repr;
-  rewrite (l0_context_perm l0_context l0_context_repr) 
-    as (context_perm ctxt repr);
-
-  ctxt
-}
-```
-
-```pulse
-fn init_l1_ctxt (deviceIDCSR_len: US.t) (aliasKeyCRT_len: US.t) 
-                (deviceID_priv: A.larray U8.t (US.v v32us)) (deviceID_pub: A.larray U8.t (US.v v32us))
-                (aliasKey_priv: A.larray U8.t (US.v v32us)) (aliasKey_pub: A.larray U8.t (US.v v32us)) 
-                (deviceIDCSR: A.larray U8.t (US.v deviceIDCSR_len)) (aliasKeyCRT: A.larray U8.t (US.v aliasKeyCRT_len))
-                (deviceID_label_len aliasKey_label_len: erased hkdf_lbl_len)
-                (cdi:erased (Seq.seq U8.t))
-                (repr:erased l0_record_repr_t)
-                (deviceIDCSR_ingredients:erased deviceIDCSR_ingredients_t)
-                (aliasKeyCRT_ingredients:erased aliasKeyCRT_ingredients_t)
-                (#deviceID_priv0 #deviceID_pub0 #aliasKey_priv0 #aliasKey_pub0
-                 #deviceIDCSR0 #aliasKeyCRT0:erased (Seq.seq U8.t))
-              
-  requires A.pts_to deviceID_priv deviceID_priv0 ** 
-           A.pts_to deviceID_pub deviceID_pub0 ** 
-           A.pts_to aliasKey_priv aliasKey_priv0 ** 
-           A.pts_to aliasKey_pub aliasKey_pub0 ** 
-           A.pts_to deviceIDCSR deviceIDCSR0 **
-           A.pts_to aliasKeyCRT aliasKeyCRT0 **
-           pure (
-            valid_hkdf_ikm_len dice_digest_len
-                       /\ aliasKey_functional_correctness
-                            dice_hash_alg dice_digest_len cdi repr.fwid
-                            aliasKey_label_len repr.aliasKey_label 
-                            aliasKey_pub0 aliasKey_priv0
-                       /\ deviceIDCSR_functional_correctness 
-                            dice_hash_alg dice_digest_len cdi
-                            deviceID_label_len repr.deviceID_label deviceIDCSR_ingredients 
-                            deviceIDCSR_len deviceIDCSR0 
-                       /\ aliasKeyCRT_functional_correctness 
-                            dice_hash_alg dice_digest_len cdi repr.fwid
-                            deviceID_label_len repr.deviceID_label aliasKeyCRT_ingredients 
-                            aliasKeyCRT_len aliasKeyCRT0 aliasKey_pub0
-           )
-  returns ctxt:context_t
-  ensures 
-    A.pts_to deviceID_priv deviceID_priv0 ** 
-    A.pts_to deviceID_pub deviceID_pub0 **
-    A.pts_to aliasKey_priv aliasKey_priv0 ** 
-    A.pts_to aliasKey_pub aliasKey_pub0 ** 
-    A.pts_to deviceIDCSR deviceIDCSR0 **
-    A.pts_to aliasKeyCRT aliasKeyCRT0 **
-    (exists* l1repr. 
-      context_perm ctxt l1repr **
-      pure (l1repr ==
-            L1_context_repr (mk_l1_context_repr_t 
-                              deviceID_label_len aliasKey_label_len deviceID_priv0 deviceID_pub0
-                              aliasKey_priv0 aliasKey_pub0 aliasKeyCRT_len aliasKeyCRT0 deviceIDCSR_len
-                              deviceIDCSR0 cdi repr deviceIDCSR_ingredients aliasKeyCRT_ingredients))
-    )
-
-{
-  let deviceID_pub_buf = A.alloc 0uy v32us;
-  let deviceID_priv_buf = A.alloc 0uy v32us;
-  let aliasKey_priv_buf = A.alloc 0uy v32us;
-  let aliasKey_pub_buf = A.alloc 0uy v32us;
-  let deviceIDCSR_buf = A.alloc 0uy deviceIDCSR_len;
-  let aliasKeyCRT_buf = A.alloc 0uy aliasKeyCRT_len;
-  memcpy v32us deviceID_priv deviceID_priv_buf;
-  memcpy v32us deviceID_pub deviceID_pub_buf;
-  memcpy v32us aliasKey_priv aliasKey_priv_buf;
-  memcpy v32us aliasKey_pub aliasKey_pub_buf;
-  memcpy deviceIDCSR_len deviceIDCSR deviceIDCSR_buf;
-  memcpy aliasKeyCRT_len aliasKeyCRT aliasKeyCRT_buf;
-
-  let l1_context = mk_l1_context_t 
-    deviceID_priv_buf deviceID_pub_buf aliasKey_priv_buf aliasKey_pub_buf 
-    aliasKeyCRT_buf deviceIDCSR_buf;
-  let l1_context_repr = hide (mk_l1_context_repr_t 
-    deviceID_label_len aliasKey_label_len deviceID_priv0 deviceID_pub0
-    aliasKey_priv0 aliasKey_pub0 aliasKeyCRT_len aliasKeyCRT0 deviceIDCSR_len
-    deviceIDCSR0 cdi repr deviceIDCSR_ingredients aliasKeyCRT_ingredients);
-
-  rewrite each deviceID_priv_buf  as l1_context.deviceID_priv,
-          deviceID_pub_buf  as l1_context.deviceID_pub,
-          aliasKey_priv_buf as l1_context.aliasKey_priv,
-          aliasKey_pub_buf  as l1_context.aliasKey_pub,
-          deviceIDCSR_buf   as l1_context.deviceIDCSR,
-          aliasKeyCRT_buf   as l1_context.aliasKeyCRT;
-
-  fold (l1_context_perm l1_context l1_context_repr);
-
-  let ctxt = mk_context_t_l1 l1_context;
-  let repr = mk_context_repr_t_l1 l1_context_repr;
-  rewrite (l1_context_perm l1_context l1_context_repr) as (context_perm ctxt repr);
-  ctxt  
-}
-```
-
-(*
-  InitializeContext: Part of DPE API 
-  Create a context in the initial state (engine context) and store the context
-  in the current session's context table. Return the context handle upon
-  success and None upon failure. 
-*)
-```pulse
-fn initialize_context'
-  (#p:perm) (#uds_bytes:Ghost.erased (Seq.seq U8.t))
-  (sid:sid_t) (uds:A.larray U8.t (US.v uds_len)) 
-                       
-  requires A.pts_to uds #p uds_bytes
-  returns _:option ctxt_hndl_t
-  ensures A.pts_to uds #p uds_bytes
-{
-  rewrite emp as (session_state_perm InUse);
-  let st = take_session_state sid InUse;
-  match st 
-  {
-    None ->
-    {
-      with s. rewrite (session_state_perm s) as emp;
-      None #ctxt_hndl_t
-    }
-    
-    Some st ->
-    {
-      if SessionStart? st 
-      {
-        rewrite (session_state_perm st) as emp;
-        let ctxt = init_engine_ctxt uds;
-        let ctxt_hndl = prng ();
-        let st' = intro_session_state_perm_available ctxt ctxt_hndl;
-        let st'' = take_session_state sid st';
-        //TODO: prove that st'' is InUse
-        drop_ (session_state_perm (dflt st'' st'));
-        Some ctxt_hndl
-      }
-      else //session error
-      {
-        destroy_session_state st;
-        rewrite emp as (session_state_perm SessionError);
-        let st' = take_session_state sid SessionError;
-        //TODO: prove st' is InUse
-        drop_ (session_state_perm (dflt st' SessionError));
-        None #ctxt_hndl_t
-      }
-    }
-  }
-}
-```
-
-let initialize_context = initialize_context'
-
-(*
-  RotateContextHandle: Part of DPE API 
-  Invalidate the current context handle and replace it with a new context
-  handle. Return the context handle upon success and None upon failure.
-*)
-```pulse
-fn rotate_context_handle' (sid:sid_t) (ctxt_hndl:ctxt_hndl_t)
-  requires emp
-  returns _:option ctxt_hndl_t
-  ensures emp
-{
-  rewrite emp as (session_state_perm InUse);
-  let st = take_session_state sid InUse;
-  match st 
-  {
-    None ->
-    {
-      with s. rewrite (session_state_perm s) as emp;
-      None #ctxt_hndl_t
-    }
-
-    Some st ->
-    {
-      if InUse? st
-      { //block concurrent access
-        rewrite (session_state_perm st) as emp;
-        None #ctxt_hndl_t
-      }
-      else if not (Available? st)
-      { //session error
-        rewrite (session_state_perm st) as emp;
-        rewrite emp as (session_state_perm SessionError);
-        let st' = take_session_state sid SessionError;
-        //TODO: prove st' is InUse
-        drop_ (session_state_perm (dflt st' SessionError));
-        None #ctxt_hndl_t
-      }
-      else 
-      {
-        let new_ctxt_hndl = prng ();
-        elim_session_state_perm_available st;
-        let st' = intro_session_state_perm_available (ctxt_of st) new_ctxt_hndl;
-        let st'' = take_session_state sid st';
-        //TODO: prove st'' is InUse
-        drop_ (session_state_perm (dflt st'' st'));
-        Some new_ctxt_hndl
-      }      
-    }
-  }
-}
-```
-let rotate_context_handle = rotate_context_handle'
-
-let maybe_context_perm (o:option context_t) =
-  match o with
-  | None -> emp
-  | _ -> exists* repr. context_perm (Some?.v o) repr
-
-```pulse
-fn intro_maybe_context_perm (c:context_t)
-  requires context_perm c 'repr
-  returns o:option context_t
-  ensures maybe_context_perm o
-{
-  rewrite (context_perm c 'repr)
-       as (context_perm (Some?.v (Some c)) 'repr);
-  fold (maybe_context_perm (Some c));
-  Some c
-}
-```
-
-```pulse
-ghost
-fn elim_maybe_context_perm (c:context_t)
-  requires maybe_context_perm (Some c)
-  ensures exists* repr. context_perm c repr
-{
-  unfold (maybe_context_perm (Some c));
-  with x y. rewrite (context_perm x y) as (context_perm c y)
-}
-```
-
-```pulse
-fn derive_child_from_context
-    (context:context_t)
-    (record:record_t)
-  requires
-    record_perm record p 'record_repr **
-    context_perm context 'context_repr
-  returns res:option context_t
-  ensures
-    record_perm record p 'record_repr **
-    context_perm context 'context_repr **
-    maybe_context_perm res
-{
-  match context
-  {
-    Engine_context c ->
-    {
-      if not (Engine_record? record)
-      { //illegal argument; reject
-        rewrite emp as (maybe_context_perm None);
-        None #context_t
-      }
-      else
-      {
-        rewrite each context as (Engine_context c);
-        let uds = get_engine_context_perm c 'context_repr;
-        // rewrite (context_perm (E) ctxt_repr) as (engine_context_perm c);
-        unfold (engine_context_perm c uds);
-        match record
-        {
-          Engine_record r ->
-          {
-            rewrite each record as (Engine_record r);
-            let r0 = get_engine_record_perm r 'record_repr p;
-            let cdi = A.alloc 0uy dice_digest_len;
-            let ret = EngineCore.engine_main cdi c.uds r;
-            with s. assert (A.pts_to cdi s);
-            fold (engine_context_perm c uds);
-            rewrite (engine_context_perm c uds)
-                 as (context_perm context 'context_repr);
-            match ret 
-            {
-              DICE_SUCCESS ->
-              {
-                let l0_ctxt = init_l0_ctxt cdi #r0 #s #uds ();
-                rewrite (engine_record_perm r p r0)
-                     as (record_perm record p 'record_repr);
-                let l0_ctxt_opt = intro_maybe_context_perm l0_ctxt;
-                l0_ctxt_opt
-              }
-
-              DICE_ERROR ->
-              {
-                A.zeroize dice_digest_len cdi;
-                A.free cdi;
-                rewrite (engine_record_perm r p r0)
-                     as (record_perm record p 'record_repr);
-                rewrite emp as (maybe_context_perm None);
-                None #context_t
-              }
-            }
-          }
-        }
-      }
-    }
-    L0_context c ->
-    { 
-      if not (L0_record? record)
-      { //illegal argument; reject
-        rewrite emp as (maybe_context_perm None);
-        None #context_t
-      }
-      else
-      {
-        match record 
-        {
-          L0_record r ->
-          {
-            // NOTE: we won't eventually release l0_context_perm because we won't 
-            // own it anymore -- we will free the cdi array
-            rewrite each context as (L0_context c);
-            let cr = get_l0_context_perm c 'context_repr;
-            unfold (l0_context_perm c cr);
-            with s. assert (A.pts_to c.cdi s);
-
-            rewrite each record as (L0_record r);
-            let r0 = get_l0_record_perm r 'record_repr p;
-
-            let idcsr_ing = r.deviceIDCSR_ingredients;
-            let akcrt_ing = r.aliasKeyCRT_ingredients;
-
-            let deviceIDCRI_len = len_of_deviceIDCRI  idcsr_ing.version idcsr_ing.s_common 
-                                                      idcsr_ing.s_org idcsr_ing.s_country;
-            let aliasKeyTBS_len = len_of_aliasKeyTBS  akcrt_ing.serialNumber akcrt_ing.i_common 
-                                                      akcrt_ing.i_org akcrt_ing.i_country 
-                                                      akcrt_ing.s_common akcrt_ing.s_org 
-                                                      akcrt_ing.s_country akcrt_ing.l0_version;
-            let deviceIDCSR_len = length_of_deviceIDCSR deviceIDCRI_len;
-            let aliasKeyCRT_len = length_of_aliasKeyCRT aliasKeyTBS_len;
-
-            let mut deviceID_pub = [| 0uy; v32us |];
-            let mut deviceID_priv = [| 0uy; v32us |];
-            let mut aliasKey_pub = [| 0uy; v32us |];
-            let mut aliasKey_priv = [| 0uy; v32us |];
-            let mut deviceIDCSR = [| 0uy; deviceIDCSR_len |];
-            let mut aliasKeyCRT = [| 0uy; aliasKeyCRT_len |];
-            
-            L0Core.l0_main  c.cdi deviceID_pub deviceID_priv 
-                            aliasKey_pub aliasKey_priv 
-                            aliasKeyTBS_len aliasKeyCRT_len aliasKeyCRT 
-                            deviceIDCRI_len deviceIDCSR_len deviceIDCSR r;
-            fold (l0_context_perm c cr);
-            rewrite (l0_context_perm c cr)
-                 as (context_perm context 'context_repr);
-            rewrite (l0_record_perm r p r0)
-                 as (record_perm record p 'record_repr);
-            let l1_context = init_l1_ctxt 
-                        deviceIDCSR_len aliasKeyCRT_len deviceID_priv deviceID_pub
-                        aliasKey_priv aliasKey_pub deviceIDCSR aliasKeyCRT
-                        (hide r.deviceID_label_len)
-                        (hide r.aliasKey_label_len) s r0 (hide idcsr_ing) (hide akcrt_ing);
-            intro_maybe_context_perm l1_context
-          }
-        }
-      }
-    }
-    L1_context _ ->
-    {
-      // ERROR - cannot invoke DeriveChild with L1 context
-      rewrite emp as (maybe_context_perm None);
-      None #context_t
-    }
-  }
-}
-```
-
-
-(*
-  DeriveChild: Part of DPE API 
-  Execute the DICE layer associated with the current context and produce a 
-  new context. Destroy the current context in the current session's context table 
-  and store the new context in the table. Return the new context handle upon
-  success and None upon failure. 
-*)
-```pulse
-fn derive_child' (sid:sid_t) (ctxt_hndl:ctxt_hndl_t) (record:record_t)
-                 (#repr:erased repr_t) (#p:perm)
-  requires record_perm record p repr
-  returns _:option ctxt_hndl_t
-  ensures record_perm record p repr
-{
-  rewrite emp as (session_state_perm InUse);
-  let st = take_session_state sid InUse;
-  match st 
-  {
-    None ->
-    {
-      with s. rewrite (session_state_perm s) as emp;
-      None #ctxt_hndl_t
-    }
-
-    Some st ->
-    {
-      if InUse? st
-      { //block concurrent access
-        rewrite (session_state_perm st) as emp;
-        None #ctxt_hndl_t
-      }
-      else if not (Available? st)
-      { //session error
-        rewrite (session_state_perm st) as emp;
-        rewrite emp as (session_state_perm SessionError);
-        let st' = take_session_state sid SessionError;
-        //TODO: prove st' is InUse
-        drop_ (session_state_perm (dflt st' SessionError));
-        None #ctxt_hndl_t
-      }
-      else 
-      {
-        elim_session_state_perm_available st;
-        let next_ctxt = derive_child_from_context (ctxt_of st) record;
-        destroy_ctxt (ctxt_of st);
-        match next_ctxt
-        {
-          None ->
-          {
-            rewrite emp as (session_state_perm SessionError);
-            rewrite (maybe_context_perm next_ctxt) as emp;
-            let st' = take_session_state sid SessionError;
-            //TODO: prove st' is InUse
-            drop_ (session_state_perm (dflt st' SessionError));
-            None #ctxt_hndl_t
-          }
-
-          Some next_ctxt ->
-          {
-            elim_maybe_context_perm next_ctxt;
-            let next_ctxt_hndl = prng();
-            let st' = intro_session_state_perm_available next_ctxt next_ctxt_hndl;
-            let st'' = take_session_state sid st';
-            //TODO: prove st'' is InUse
-            drop_ (session_state_perm (dflt st'' st'));
-            Some next_ctxt_hndl
-          }
-        }
-      }
-    }
-  }
-}
-```
-let derive_child = derive_child'
+//           Some next_ctxt ->
+//           {
+//             elim_maybe_context_perm next_ctxt;
+//             let next_ctxt_hndl = prng();
+//             let st' = intro_session_state_perm_available next_ctxt next_ctxt_hndl;
+//             let st'' = take_session_state sid st';
+//             //TODO: prove st'' is InUse
+//             drop_ (session_state_perm (dflt st'' st'));
+//             Some next_ctxt_hndl
+//           }
+//         }
+//       }
+//     }
+//   }
+// }
+// ```
+// let derive_child = derive_child'
