pulse/share/steel/examples/pulse/dice/dpe/DPE.fsti
@@ -35,32 +35,32 @@ val ctxt_hndl_t : eqtype
 let sid_t : eqtype = U32.t // FIXME: type needed by DPE_CBOR
 
 
-val get_profile () : stt profile_descriptor_t emp (fun _ -> emp)
+// val get_profile () : stt profile_descriptor_t emp (fun _ -> emp)
 
-val open_session () : stt (option sid_t) emp (fun _ -> emp)
+// val open_session () : stt (option sid_t) emp (fun _ -> emp)
 
-val destroy_context (sid:sid_t) (ctxt_hndl:ctxt_hndl_t) : stt bool emp (fun _ -> emp)
+// val destroy_context (sid:sid_t) (ctxt_hndl:ctxt_hndl_t) : stt bool emp (fun _ -> emp)
 
-val close_session (sid:sid_t) : stt bool emp (fun _ -> emp)
+// val close_session (sid:sid_t) : stt bool emp (fun _ -> emp)
 
-val initialize_context (#p:perm)
-                       (#uds_bytes:erased (Seq.seq U8.t))
-                       (sid:sid_t) 
-                       (uds:A.larray U8.t (US.v uds_len))         
-  : stt (option ctxt_hndl_t) 
-        (A.pts_to uds #p uds_bytes)
-        (fun _ -> A.pts_to uds #p uds_bytes)
+// val initialize_context (#p:perm)
+//                        (#uds_bytes:erased (Seq.seq U8.t))
+//                        (sid:sid_t) 
+//                        (uds:A.larray U8.t (US.v uds_len))         
+//   : stt (option ctxt_hndl_t) 
+//         (A.pts_to uds #p uds_bytes)
+//         (fun _ -> A.pts_to uds #p uds_bytes)
 
-val rotate_context_handle (sid:sid_t)
-                          (ctxt_hndl:ctxt_hndl_t)
-  : stt (option ctxt_hndl_t) emp (fun _ -> emp)
+// val rotate_context_handle (sid:sid_t)
+//                           (ctxt_hndl:ctxt_hndl_t)
+//   : stt (option ctxt_hndl_t) emp (fun _ -> emp)
 
-val derive_child (sid:sid_t)
-                 (ctxt_hndl:ctxt_hndl_t)
-                 (record:record_t)
-                 (#repr:erased repr_t)
-                 (#p:perm)
-  : stt (option ctxt_hndl_t) 
-        (record_perm record p repr)
-        (fun _ -> record_perm record p repr)
+// val derive_child (sid:sid_t)
+//                  (ctxt_hndl:ctxt_hndl_t)
+//                  (record:record_t)
+//                  (#repr:erased repr_t)
+//                  (#p:perm)
+//   : stt (option ctxt_hndl_t) 
+//         (record_perm record p repr)
+//         (fun _ -> record_perm record p repr)
 
