pulse/share/steel/examples/pulse/lib/Pulse.Lib.Mutex.fsti
@@ -17,7 +17,7 @@
 module Pulse.Lib.Mutex
 open Pulse.Lib.Core
 
-module B = Pulse.Lib.Box
+open Pulse.Lib.Reference
 
 //
 // A model of Rust mutex
@@ -36,14 +36,14 @@ val new_mutex (#a:Type0) (p:a -> vprop) (x:a)
         (requires p x)
         (ensures fun _ -> emp)
 
-val belongs_to_mutex (#a:Type0) (#p:a -> vprop) (r:B.box a) (m:mutex p) : vprop
+val belongs_to_mutex (#a:Type0) (#p:a -> vprop) (r:ref a) (m:mutex p) : vprop
 
 val lock (#a:Type0) (#p:a -> vprop) (m:mutex p)
-  : stt (B.box a)
+  : stt (ref a)
         (requires emp)
-        (ensures fun r -> r `belongs_to_mutex` m ** (exists* v. B.pts_to r v ** p v))
+        (ensures fun r -> r `belongs_to_mutex` m ** (exists* v. pts_to r v ** p v))
 
-val unlock (#a:Type0) (#p:a -> vprop) (m:mutex p) (r:B.box a)
+val unlock (#a:Type0) (#p:a -> vprop) (m:mutex p) (r:ref a)
   : stt unit
-        (requires r `belongs_to_mutex` m ** (exists* v. B.pts_to r v ** p v))
+        (requires r `belongs_to_mutex` m ** (exists* v. pts_to r v ** p v))
         (ensures fun _ -> emp)
